Ugly comments to be rewritten

coq/theories/OGS/Spec.v
@@ -8,31 +8,62 @@ From OGS.ITree Require Import ITree Monad Eq.
 
 Open Scope ctx_scope.
 
-Definition delay (X : Type) : Type := itree ∅ₑ (fun _ => X) T1_0.
+(* domain of computations: isomorphic to Capretta's delay monad *)
+Definition delay (X : Type) : Type :=
+  itree ∅ₑ (fun _ => X) T1_0.
 
-Record lang_spec : Type := {
+(*
+  Mapping with pdf: operational signature
+
+typ : set of types
+msg : to each typ a message
+dom : for each message the context extension it entails (a.k.a. free variables of the message)
+ *)
+Record interaction_spec : Type := {
   typ : Type ;
   msg : typ -> Type ;
-  dom : forall t, msg t -> ctx typ ; 
+  dom : forall t, msg t -> ctx typ ;
 }.
 Arguments dom _ [_].
 
 Section a.
 
-  Context (S : lang_spec).
+  Context (S : interaction_spec).
 
+  (* pdf: msg* *)
   Definition msg' (Γ : ctx S.(typ)) : Type :=
     { t : S.(typ) & Γ ∋ t * S.(msg) t }%type.
 
+  (* pdf: dom* *)
   Definition dom' {Γ} (m : msg' Γ) : ctx S.(typ) :=
     S.(dom) (snd (projT2 m)).
 
+  (* (Axiomatization of the) Operational machine:
+
+Question GJ: should msg' be renamed into move?
+
+TODO: concretize env
+
+     1-5 : current status of the pdf
+     6-10: administration
+   *)
   Record machine : Type := {
+      (* configurations (used to be called "terms" far in the past)
+         Roughly: active states
+       *)
     conf : ctx S.(typ) -> Type ;
+      (* assignments
+         Roughly: passive states
+       *)
     env : ctx S.(typ) -> ctx S.(typ) -> Type ;
+      (* evaluation function for configurations *)
     eval {Γ} : conf Γ -> delay { m : msg' Γ & env Γ (dom' m) } ;
+      (* (very) Roughly: injecting patterns in terms *)
     emb {Γ} (m : msg' Γ) : conf (Γ +▶ dom' m) ;
+      (* substitution *)
     c_sub {Γ Δ} : conf Γ -> env Δ Γ -> conf Δ ;
+
+      (* axiomatization of the assignments *)
     e_empty {Δ} : env Δ ∅ ;
     e_cat {Γ1 Γ2 Δ} : env Δ Γ1 -> env Δ Γ2 -> env Δ (Γ1 +▶ Γ2) ;
     e_ren {Γ Δ1 Δ2} : Δ1 ⊆ Δ2 -> env Δ1 Γ -> env Δ2 Γ ;
@@ -40,12 +71,23 @@ Section a.
     e_id {Γ} : env Γ Γ ;
   }.
 
-  Definition sub_eval_msg {Γ Δ} (M : machine) (e : M.(env) Δ Γ) (t : M.(conf) Γ) : delay (msg' Δ) :=
-    fmap (fun _ r => projT1 r) _ (M.(eval) (M.(c_sub) t e)).      
+  Arguments it_wbisim {I E X i}.
+  Definition sub_eval_msg {Γ Δ}
+    (M : machine) (e : M.(env) Δ Γ) (t : M.(conf) Γ)
+    : delay (msg' Δ) :=
+    fmap (fun _ r => projT1 r) _ (M.(eval) (M.(c_sub) t e)).
 
-  Definition ciu (M : machine) {Γ} Δ (x y : M.(conf) Γ) : Prop :=
-    forall (e : M.(env) Δ Γ), it_wbisim _ _ _ (sub_eval_msg M e x) (sub_eval_msg M e y).
+  (* The quantification over contexts is inlined in
+     the quantification over assignments [forall (e : M.(env) Δ Γ)]
+   *)
+  Definition ciu
+    (M : machine) {Γ} Δ (x y : M.(conf) Γ) : Prop :=
+    forall (e : M.(env) Δ Γ),
+      it_wbisim (sub_eval_msg M e x) (sub_eval_msg M e y).
 
+  (* Section 3: game definition
+     ↓+ ~ join_even
+   *)
   Definition alt_ext : Type := ctx (ctx S.(typ)).
 
   Definition ogs_hg : half_game alt_ext alt_ext := {|
@@ -59,31 +101,70 @@ Section a.
 
   Definition ogs_e : event alt_ext alt_ext := e_of_g ogs_g.
 
-  Inductive alt_env (M : machine) (Δ : ctx S.(typ)) : bool -> alt_ext -> Type :=
+  Notation player   := true.
+  Notation opponent := false.
+  (* Env* (def 3.12)
+     Env M Δ player es : environment part of the player (aka active at es) configuration at (Δ + es)
+     Env M Δ opponent es : environment part of the opponent (aka passive at es) configuration at (Δ + es)
+   *)
+  Inductive alt_env (M : machine) (Δ : ctx S.(typ))
+    : bool -> alt_ext -> Type :=
   | ENil {b} : alt_env M Δ b ∅
-  | EConT {a Γ} : alt_env M Δ false a
-                  -> alt_env M Δ true (a ▶ Γ)
-  | EConF {a Γ} : alt_env M Δ true a
+  | EConT {a Γ} : alt_env M Δ opponent a
+                  -> alt_env M Δ player (a ▶ Γ)
+  | EConF {a Γ} : alt_env M Δ player a
                   -> M.(env) (Δ +▶ join_even a) Γ
-                  -> alt_env M Δ false (a ▶ Γ)
+                  -> alt_env M Δ opponent (a ▶ Γ)
   .
   Arguments ENil {M Δ b}.
   Arguments EConT {M Δ a Γ}.
   Arguments EConF {M Δ a Γ}.
 
-  Equations concat0 {M Δ b a} : alt_env M Δ b a
-             -> M.(env) (Δ +▶ join_even_odd_aux b a) (join_even_odd_aux (negb b) a) :=
+  (* flattens an alternating environment into an unstructured one *)
+  Equations concat0 {M Δ b a} :
+    alt_env M Δ b a ->
+    M.(env)
+        (Δ +▶ join_even_odd_aux b a)
+        (join_even_odd_aux (negb b) a) :=
     concat0 (ENil) := M.(e_empty) ;
     concat0 (EConT u) := M.(e_ren) (r_concat3_1 _ _ _) (concat0 u) ;
     concat0 (EConF u e) := M.(e_cat) (concat0 u) e .
 
-  Definition concat1 {M Δ a} b : alt_env M Δ true a
-             -> alt_env M Δ false a -> M.(env) Δ (join_even_odd_aux b a).
-    revert b; induction a; intros b u v; dependent destruction u; dependent destruction v.
-    - refine (M.(e_empty)).
-    - destruct b; cbn in *.
+  (* Flattens a pair of alternating environments for resp. player and opponent into a "closed" substitution
+   *)
+  Definition concat1 {M Δ a} b :
+    alt_env M Δ player a ->
+    alt_env M Δ opponent a ->
+    M.(env) Δ (join_even_odd_aux b a).
+    revert b; induction a.
+    - intros b u v.
+      exact (M.(e_empty)).
+    - intros b u v.
+      dependent destruction u.
+      dependent destruction v.
+      destruct b; cbn in *.
       * refine (M.(e_cat) (IHa false v u) _).
         refine (M.(e_comp) _ e).
         refine (M.(e_cat) M.(e_id) (IHa true v u)).
       * exact (IHa true v u).
-   Qed.
+  Defined.
+
+  Lemma quatre_six_un {M Δ a}
+    (u : alt_env M Δ player a)
+    (v : alt_env M Δ opponent a) :
+    M.(e_comp)
+        (M.(e_cat) M.(e_id) (concat1 player u v))
+        (concat0 u)
+    = concat1 opponent u v.
+  Admitted.
+
+  Lemma quatre_six_deux {M Δ a}
+    (u : alt_env M Δ player a)
+    (v : alt_env M Δ opponent a) :
+    M.(e_comp)
+        (M.(e_cat) M.(e_id) (concat1 opponent u v))
+        (concat0 v)
+    = concat1 player u v.
+  Admitted.
+
+
